ott_coq/destination_calculus_notations.v
@@ -4,13 +4,18 @@ Require Import Ott.destination_calculus_ott.
 Require Import Ott.ext_nat.
 
 (* Var, holes and dests names : 15-19 *)
-Notation "⋆" := (nil).
-Notation "d '.1'" := (d ++ (cons 1 nil)) (at level 18, right associativity).
-Notation "d '.2'" := (d ++ (cons 2 nil)) (at level 18, right associativity).
-Notation "d '.3'" := (d ++ (cons 3 nil)) (at level 18, right associativity).
+Notation "'ʰmax(' b , .. , c ')'" := (hdns_from_list (cons b .. (cons c nil) ..)) (at level 0, no associativity).
 
-Notation "'dyn' d" := (hdn_D d) (at level 19, no associativity).
-Notation "'static' hdn" := (hdn_S hdn) (at level 19, no associativity).
+(* Hole names sets : 20-24 *)
+Notation "'ʰ{' b , .. , c '}'" := (hdns_from_list (cons b .. (cons c nil) ..)) (at level 0, no associativity).
+Notation "H1 '∪' H2" := (HdnsM.union H1 H2) (at level 24, left associativity, H2 at next level).
+Notation "H 'ʰ⩲' h" := (hdns_incr_hnames H h) (at level 20, h at level 19, no associativity).
+Notation "'ᶜhnames(' G ')'" := (hdns_from_ctx G) (at level 0, no associativity).
+Notation "'ᵉhnames(' C ')'" := (hdns_from_ectx C) (at level 0, no associativity).
+
+(* Var names : 15-19 *)
+
+(* Mode names : 25-29 *)
 
 (* Multiplicities : 25-29 *)
 Notation "'¹ν'" := (Some (pair Lin (Fin 0))).
@@ -33,59 +38,62 @@ Notation "! m '⁔' T" := (type_E m T) (at level 30, m at level 29, right associ
 Notation "T ⧔ U" := (type_A T U) (at level 55, left associativity, U at next level).
 Notation "T '⁔' m '→' U" := (type_F T m U) (at level 59, m at level 29, right associativity, U at level 59).
 Notation "⌊ T ⌋ m" := (type_D T m) (at level 35, T at level 59, m at level 29, no associativity).
+Notation "T '↣' U" := (type_C T U) (at level 59, no associativity, U at level 59).
 
 (* Values : 30-59 *)
 Notation "'ᵛ-' h" := (val_H h) (at level 31, h at level 19, no associativity).
 Notation "'ᵛ+' h" := (val_D h) (at level 31, h at level 19, no associativity).
 Notation "'ᵛ()'" := (val_U).
-Notation "'λ' x ⟼ t" := (val_F x t) (at level 59, x at level 19, t at level 59, right associativity).
+Notation "'λᵛ' x ⟼ t" := (val_F x t) (at level 59, x at level 19, t at level 59, right associativity).
 Notation "'Inl' v" := (val_L v) (at level 31, right associativity, v at level 31).
 Notation "'Inr' v" := (val_R v) (at level 31, right associativity, v at level 31).
 Notation "'ᴇ' m '⁔' v" := (val_E m v) (at level 31, m at level 29, v at level 31, right associativity).
 Notation "'ᵛ(' v ',' w ')'" := (val_P v w) (at level 0, v at level 59, w at level 59, no associativity).
-Notation "'⟨' v '❟' w '⟩' D" := (val_A v w D) (at level 31, no associativity, v at level 59, w at level 59, D at next level).
-Notation "v 'ᵉ[' f ]" := (val_hfill v f) (at level 30, f at level 64, no associativity).
+Notation "H '⟨' v '❟' w '⟩'" := (val_A H v w) (at level 31, no associativity, v at level 59, w at level 59).
+Notation "v 'ᵛ⩲' h " := (val_incr_hnames v h) (at level 30, h at level 19, no associativity).
 
 (* Terms : 40-59 *)
 Notation "t ≻ u" := (term_App t u) (at level 42, left associativity, u at next level).
-Notation "t 'ᵗ;' u" := (term_PatU t u) (at level 45, left associativity, u at next level).
-Notation "t '≻case' 'ᵛ{' 'Inl' x1 ⟼ u1 , 'Inr' x2 ⟼ u2 '}'" := (term_PatS t x1 u1 x2 u2) (at level 59, x1 at level 19, x2 at level 19, u1 at level 59, u2 at level 59, right associativity).
-Notation "t '≻case' 'ᵛ(' x1 ',' x2 ')' ⟼ u" := (term_PatP t x1 x2 u) (at level 59, x1 at level 19, x2 at level 19, u at level 59, right associativity).
-Notation "t '≻case' 'ᴇ' m '⁔' x ⟼ u" := (term_PatE t m x u) (at level 59, m at level 29, x at level 19, u at level 59, right associativity).
+Notation "t 'ₜ;' u" := (term_PatU t u) (at level 45, left associativity, u at next level).
+Notation "t '≻case' m '{Inl' x1 ⟼ u1 , 'Inr' x2 ⟼ u2 '}'" := (term_PatS t m x1 u1 x2 u2) (at level 59, m at level 29, x1 at level 19, x2 at level 19, u1 at level 59, u2 at level 59, right associativity).
+Notation "t '≻case' m 'ᵛ(' x1 ',' x2 ')' ⟼ u" := (term_PatP t m x1 x2 u) (at level 59, m at level 29, x1 at level 19, x2 at level 19, u at level 59, right associativity).
+Notation "t '≻case' m 'ᴇ' n '⁔' x ⟼ u" := (term_PatE t m n x u) (at level 59,  m at level 29, n at level 29, x at level 19, u at level 59, right associativity).
 Notation "t '≻map' x ⟼ u" := (term_Map t x u) (at level 59, x at level 19, u at level 59, right associativity).
 Notation "'to⧔' t" := (term_ToA t) (at level 41, right associativity, t at level 41).
 Notation "'from⧔' t" := (term_FromA t) (at level 41, right associativity, t at level 41).
 Notation "'alloc' T" := (term_Alloc T) (at level 40, no associativity, T at next level).
 Notation "t ⨞ 'ᵛ()'" := (term_FillU t) (at level 43, left associativity).
+Notation "t ⨞ 'λ' x ⟼ u" := (term_FillF t x u) (at level 43, x at level 19, u at next level, left associativity).
 Notation "t ⨞ 'Inl'" := (term_FillL t) (at level 43, left associativity).
 Notation "t ⨞ 'Inr'" := (term_FillR t) (at level 43, left associativity).
 Notation "t ⨞ 'ᵛ(,)'" := (term_FillP t) (at level 43, left associativity).
 Notation "t ⨞ 'ᴇ' m" := (term_FillE t m) (at level 43, left associativity, m at level 29).
 Notation "t '⨞·' u" := (term_FillC t u) (at level 43, left associativity, u at next level).
-Notation "t 'ᵗ[' x '≔' v ]" := (term_sub t x v) (at level 40, x at level 19, v at level 59, left associativity).
+Notation "t 'ˢ[' x '≔' v ]" := (term_sub t x v) (at level 40, x at level 19, v at level 59, left associativity).
 
 (* Bindings and contexts : 60 - 64 *)
 Notation "'ᵛ' x 'ː' m '‗' T" := (bndr_V x m T) (at level 60, x at level 19, m at level 29, T at level 59, no associativity).
 Notation "'⁺' h 'ː' m ⌊ T ⌋ n" := (bndr_D h m T n) (at level 60, h at level 19, m at level 29, T at level 59, n at level 29, no associativity).
-Notation "'⁻' h 'ː' n '‗' T" := (bndr_H h n T) (at level 60, h at level 19, n at level 29, T at level 59, no associativity).
+Notation "'⁻' h 'ː' T '‗' n" := (bndr_H h T n) (at level 60, h at level 19, n at level 29, T at level 59, no associativity).
 
 Notation "'ᶜ{' b , .. , c '}'" := (ctx_from_list (cons b .. (cons c nil) ..)) (at level 0, no associativity).
 Notation "m 'ᶜ·' G" := (ctx_stimes m G) (at level 62, G at level 62, right associativity).
 Notation "G '⨄' H" := (ctx_union G H) (at level 63, left associativity, H at next level).
-Notation "G '⁻⨄⁺' H" := (ctx_interact G H) (at level 63, no associativity, H at next level).
 Notation "ᶜ- G" := (ctx_minus G) (at level 61, no associativity, G at next level).
 
-(* Effects : 60-64 *)
-Notation "'ε'" := nil.
-Notation "h '≔' v" := (hf_F h v) (at level 60, v at level 59, no associativity).
-Infix "»" := app (at level 61, right associativity).
+(* Evaluation contexts and extended terms : 65-69 *)
+
+Notation "'ᵉ[' ]" := ectx_Id.
+Notation "H 'ᵒ⟨' v1 '❟' C" := (ectx_AOpen H v1 C) (at level 66, v1 at level 59, C at level 66, right associativity).
+Notation "C '∘' D" := (ectx_Comp C D) (at level 67, D at level 67, right associativity).
+Notation "C 'ᶠ[' h '≔' H '‗' v ]" := (ectx_fill C h H v) (at level 65, h at level 19, H at level 24, v at level 59, left associativity).
+
+Notation "C 'ʲ[' t ]" := (eterm_ECtxApp C t) (at level 65, t at level 59, no associativity).
 
 (* Typing and semantics : 70 - 79 *)
-Notation "G 'ᵉ⫦' e" := (TyR_eff G e) (at level 70, e at level 64, no associativity).
-Notation "G 'ᵉ⊢' e" := (Ty_eff G e) (at level 70, e at level 64, no associativity).
-Notation "G 'ᵗ⫦' t 'ː' T" := (TyR_term G t T) (at level 70, t at level 59, T at level 59, no associativity).
-Notation "G 'ᵗ⊢' t 'ː' T" := (Ty_term G t T) (at level 70, t at level 59, T at level 59, no associativity).
-Notation "G 'ᶜ⊢' v ⋄ e 'ː' T" := (Ty_cmd G v e T) (at level 70, v at level 59, e at level 64, T at level 59, no associativity).
+Notation "G 'ᵛ⫦' v 'ː' T" := (TyR_val G v T) (at level 70, v at level 59, T at level 59, no associativity).
+Notation "G 'ᵗ⊢' j 'ː' T" := (Ty_term G j T) (at level 70, j at level 69, T at level 59, no associativity).
+Notation "G 'ᵉ⫦' C 'ː' T" := (TyR_ectx G C T) (at level 70, C at level 69, T at level 59, no associativity).
 
-Notation "v1 '‿' D1 | e1 '⤋' v2 '‿' D2 | e2" := (Sem_eff v1 D1 e1 v2 D2 e2) (at level 70, D1 at level 64, e1 at level 64, v2 at level 59, D2 at level 64, e2 at level 64, no associativity).
-Notation "t '‿' d '⇓' v ⋄ e" := (Sem_term t d v e) (at level 70, d at level 19, v at level 59, e at level 64, no associativity).
+Notation "j ⟶ k" := (Sem_eterm j k) (at level 70, k at level 69, no associativity).
+
